fstar/new/Test.TreeKEM.fst
@@ -6,6 +6,7 @@ open Test.Types
 open Test.Utils
 open Tree
 open TreeSync
+open TreeSync.Hash
 open TreeKEM
 open TreeSyncTreeKEMBinder
 open NetworkTypes
@@ -14,6 +15,8 @@ open Lib.Result
 open Test.Utils
 open Lib.ByteSequence
 open Crypto
+
+module TreeMath = TreeMath
 
 val find_my_index: #l:nat -> #n:tree_size l -> treesync l n -> key_package_nt -> ML (res:nat{res<n})
 let find_my_index #l #n t kp =
@@ -30,6 +33,38 @@ let find_my_index #l #n t kp =
   let res = extract_option "couldn't find my_index" (find_first test (Seq.seq_to_list (tree_membership t))) in
   res
 
+val gen_treekem_output: ciphersuite -> treekem_test_input -> ML treekem_test_output
+let gen_treekem_output cs t =
+  let my_key_package = extract_option "bad key package" ((ps_to_pse ps_key_package).parse_exact (hex_string_to_bytes t.my_key_package)) in
+  let ratchet_tree = extract_option "bad ratchet tree" ((ps_to_pse ps_ratchet_tree).parse_exact (hex_string_to_bytes t.ratchet_tree_before)) in
+  let my_leaf_secret = (hex_string_to_bytes t.my_leaf_secret) in
+  let my_path_secret = (hex_string_to_bytes t.my_path_secret) in
+  let add_sender = FStar.UInt32.v t.add_sender in
+  let (|l, n|) = extract_result (ratchet_tree_l_n ratchet_tree) in
+  let ts0 = extract_result (ratchet_tree_to_treesync l n ratchet_tree) in
+  let tk0 = extract_result (treesync_to_treekem cs ts0) in
+  let my_index = find_my_index ts0 my_key_package in
+  if not (my_index <> add_sender) then
+    failwith ("new leaf cannot be equal to add_sender: my_index=" ^ nat_to_string my_index ^ " add_sender=" ^ nat_to_string add_sender ^ "\n")
+  else if not (add_sender < n) then
+    failwith "add_sender is too big"
+  else (
+    let tree_hash_before = extract_result (tree_hash cs (TreeMath.root l) ts0) in
+    let upk0 = extract_result (mk_init_path tk0 my_index add_sender my_path_secret bytes_empty) in
+    let old_leaf_package = extract_result (key_package_to_treesync my_key_package) in
+    let ups0 = extract_result (treekem_to_treesync old_leaf_package upk0) in
+    let ts1 = apply_path dumb_credential ts0 ups0 in
+    let tk1 = extract_result (treesync_to_treekem cs ts1) in
+    let root_secret_after_add = extract_result (root_secret tk1 my_index my_leaf_secret bytes_empty) in
+    {
+      tree_hash_before = bytes_to_hex_string tree_hash_before;
+      root_secret_after_add = bytes_to_hex_string root_secret_after_add;
+      root_secret_after_update = "";
+      ratchet_tree_after = "";
+      tree_hash_after = "";
+    }
+  )
+
 val test_treekem_one: treekem_test -> ML bool
 let test_treekem_one t =
   if FStar.UInt16.v t.tk_cipher_suite <> 3 then (
@@ -43,28 +78,10 @@ let test_treekem_one t =
   end
   | Success cs -> begin
     IO.print_string "Running test!!!\n";
-    let my_key_package = extract_option "bad key package" ((ps_to_pse ps_key_package).parse_exact (hex_string_to_bytes t.my_key_package)) in
-    let ratchet_tree = extract_option "bad ratchet tree" ((ps_to_pse ps_ratchet_tree).parse_exact (hex_string_to_bytes t.ratchet_tree_before)) in
-    let my_leaf_secret = (hex_string_to_bytes t.my_leaf_secret) in
-    let my_path_secret = (hex_string_to_bytes t.my_path_secret) in
-    let add_sender = FStar.UInt32.v t.add_sender in
-    let (|l, n|) = extract_result (ratchet_tree_l_n ratchet_tree) in
-    let ts0 = extract_result (ratchet_tree_to_treesync l n ratchet_tree) in
-    let tk0 = extract_result (treesync_to_treekem cs ts0) in
-    let my_index = find_my_index ts0 my_key_package in
-    if not (my_index <> add_sender) then
-      failwith ("new leaf cannot be equal to add_sender: my_index=" ^ nat_to_string my_index ^ " add_sender=" ^ nat_to_string add_sender ^ "\n")
-    else if not (add_sender < n) then
-      failwith "add_sender is too big"
-    else (
-      let upk0 = extract_result (mk_init_path tk0 my_index add_sender my_path_secret bytes_empty) in
-      let old_leaf_package = extract_result (key_package_to_treesync my_key_package) in
-      let ups0 = extract_result (treekem_to_treesync old_leaf_package upk0) in
-      let ts1 = apply_path dumb_credential ts0 ups0 in
-      let tk1 = extract_result (treesync_to_treekem cs ts1) in
-      let root_secret_after_add = extract_result (root_secret tk1 my_index my_leaf_secret bytes_empty) in
-      (bytes_to_hex_string root_secret_after_add) = t.root_secret_after_add
-    )
+    let our_output = gen_treekem_output cs t.tk_input in
+    let tree_hash_before_ok = check_equal "tree_hash_before_ok" string_to_string t.tk_output.tree_hash_before our_output.tree_hash_before in
+    let root_secret_after_add_ok = check_equal "root_secret_after_add" string_to_string t.tk_output.root_secret_after_add our_output.root_secret_after_add in
+    tree_hash_before_ok && root_secret_after_add_ok
   end
 
 val test_treekem: list treekem_test -> ML bool
