fstar/new/Crypto.Derived.fsti
@@ -7,5 +7,7 @@ open Lib.ByteSequence
 open NetworkTypes
 
 val ciphersuite_from_nt: cipher_suite_nt -> result ciphersuite
+val ciphersuite_to_nt: ciphersuite -> result cipher_suite_nt
+
 val expand_with_label: ciphersuite -> secret:bytes -> label:bytes -> context:bytes -> len:size_nat -> result (lbytes len)
 val derive_secret: cs:ciphersuite -> secret:bytes -> label:bytes -> result (lbytes (kdf_length cs))
